progress towards FlushEquivalentLookups

disk-betree/DiskBetreeInv.dfy
@@ -220,33 +220,253 @@ abstract module DiskBetreeInv {
     }
   }
 
-  function transformLookup<Value>(lookup: Lookup<Value>, oldref: BC.Reference, newref: BC.Reference, newnode: Node) : Lookup<Value>
-  ensures |transformLookup(lookup, oldref, newref, newnode)| == |lookup|
+  function transformLookup<Value>(lookup: Lookup<Value>, key: Key, oldref: BC.Reference, newref: BC.Reference, newnode: Node) : Lookup<Value>
+  ensures |transformLookup(lookup, key, oldref, newref, newnode)| == |lookup|;
   ensures forall i :: 0 <= i < |lookup| ==>
-      transformLookup(lookup, oldref, newref, newnode)[i].ref ==
-        (if lookup[i].ref == oldref then newref else lookup[i].ref)
+      transformLookup(lookup, key, oldref, newref, newnode)[i].ref ==
+        (if lookup[i].ref == oldref then newref else lookup[i].ref);
   ensures forall i :: 0 <= i < |lookup| ==>
-      transformLookup(lookup, oldref, newref, newnode)[i].node ==
-        (if lookup[i].ref == oldref then newnode else lookup[i].node)
+      transformLookup(lookup, key, oldref, newref, newnode)[i].node ==
+        (if lookup[i].ref == oldref then newnode else lookup[i].node);
+  //ensures |lookup| > 0 ==> transformLookup(lookup, key, oldref, newref, newnode)[0].accumulatedBuffer == transformLookup(lookup, key, oldref, newref, newnode)[0].node.buffer[key]
+  //ensures (forall i :: 0 < i < |transformLookup(lookup, key, oldref, newref, newnode)| ==> transformLookup(lookup, key, oldref, newref, newnode)[i].accumulatedBuffer == transformLookup(lookup, key, oldref, newref, newnode)[i-1].accumulatedBuffer + transformLookup(lookup, key, oldref, newref, newnode)[i].node.buffer[key])
   decreases lookup
   {
     if |lookup| == 0 then
       []
     else
-      transformLookup(lookup[.. |lookup| - 1], oldref, newref, newnode) + 
-        [if lookup[|lookup| - 1].ref == oldref then Layer(newref, newnode, lookup[|lookup|-1].accumulatedBuffer) else lookup[|lookup| - 1]]
+      var pref := transformLookup(lookup[.. |lookup| - 1], key, oldref, newref, newnode);
+      var accBuf := if |pref| == 0 then [] else pref[|pref| - 1].accumulatedBuffer;
+      pref +
+        [if lookup[|lookup| - 1].ref == oldref then
+          Layer(newref, newnode, accBuf + (if key in newnode.buffer then newnode.buffer[key] else []))
+         else
+          Layer(lookup[|lookup| - 1].ref, lookup[|lookup| - 1].node, accBuf + (if key in lookup[|lookup| - 1].node.buffer then lookup[|lookup| - 1].node.buffer[key] else []))
+        ]
   }
 
-  function flushTransformLookupRev<Value>(lookup': Lookup, parentref: BC.Reference, parent: Node, childref: BC.Reference, child: Node, newchildref: BC.Reference) : Lookup
+  lemma transformLookupAccumulatesMessages<Value>(lookup: Lookup<Value>, key: Key, oldref: BC.Reference, newref: BC.Reference, newnode: Node)
+  requires |lookup| > 0
+  requires LookupVisitsWFNodes(transformLookup(lookup, key, oldref, newref, newnode))
+  ensures LookupAccumulatesMessages(key, transformLookup(lookup, key, oldref, newref, newnode))
   {
-    transformLookup(transformLookup(lookup', newchildref, childref, child), parentref, parentref, parent)
+  }
+
+  // Change every parentref in lookup to the newparent, and likewise for the child.
+  // However, when changing the child, we check first that it actually came from the parent
+  // (since there might be other pointers to child)
+  function transformLookupParentAndChild<Value>(lookup: Lookup<Value>, key: Key, parentref: BC.Reference, newparent: Node, movedKeys: iset<Key>, oldchildref: BC.Reference, newchildref: BC.Reference, newchild: Node) : Lookup<Value>
+  requires |lookup| > 0
+  ensures |transformLookupParentAndChild(lookup, key, parentref, newparent, movedKeys, oldchildref, newchildref, newchild)| == |lookup|;
+
+  /*
+  ensures transformLookupParentAndChild(lookup, key, parentref, newparent, movedKeys, oldchildref, newchildref, newchild)[0].ref == lookup[0].ref
+  ensures transformLookupParentAndChild(lookup, key, parentref, newparent, movedKeys, oldchildref, newchildref, newchild)[0].node == (if lookup[0].ref == parentref then newparent else lookup[0].node);
+
+  ensures forall i :: 0 < i < |lookup| && lookup[i].ref == oldchildref && lookup[i-1].ref == parentref && key in movedKeys ==>
+    && transformLookupParentAndChild(lookup, key, parentref, newparent, movedKeys, oldchildref, newchildref, newchild)[i].ref == newchildref
+    && transformLookupParentAndChild(lookup, key, parentref, newparent, movedKeys, oldchildref, newchildref, newchild)[i].node == newchild
+
+  ensures forall i :: 0 <= i < |lookup| && lookup[i].ref == parentref ==>
+    && transformLookupParentAndChild(lookup, key, parentref, newparent, movedKeys, oldchildref, newchildref, newchild)[i].ref == parentref
+    && transformLookupParentAndChild(lookup, key, parentref, newparent, movedKeys, oldchildref, newchildref, newchild)[i].node == newparent
+
+  ensures forall i :: 0 < i < |lookup| && lookup[i].ref != parentref && !(lookup[i].ref == oldchildref && lookup[i-1].ref == parentref && key in movedKeys) ==>
+    && transformLookupParentAndChild(lookup, key, parentref, newparent, movedKeys, oldchildref, newchildref, newchild)[i].ref == lookup[i].ref
+    && transformLookupParentAndChild(lookup, key, parentref, newparent, movedKeys, oldchildref, newchildref, newchild)[i].node == lookup[i].node
+  */
+
+  /*
+  ensures forall i :: 0 <= i < |lookup| ==>
+      transformLookupParentAndChild(lookup, key, parentref, newparent, movedKeys, oldchildref, newchildref, newchild)[i].ref ==
+        (if lookup[i].ref == parentref then parentref else
+         if lookup[i].ref == oldchildref && i > 0 && lookup[i-1].ref == parentref && key in movedKeys then newchildref else
+         lookup[i].ref)
+  ensures forall i :: 0 <= i < |lookup| ==>
+      transformLookupParentAndChild(lookup, key, parentref, newparent, movedKeys, oldchildref, newchildref, newchild)[i].node ==
+        (if lookup[i].ref == parentref then newparent else
+         if lookup[i].ref == oldchildref && i > 0 && lookup[i-1].ref == parentref && key in movedKeys then newchild else
+         lookup[i].node)
+  */
+
+  decreases lookup
+  {
+    var pref := if |lookup| > 1 then transformLookupParentAndChild(lookup[.. |lookup| - 1], key, parentref, newparent, movedKeys, oldchildref, newchildref, newchild) else [];
+
+    // these seem to be required?
+    /*
+    assert forall i :: 0 <= i < |pref| ==>
+      pref[i].ref ==
+        (if lookup[..|lookup|-1][i].ref == parentref then parentref else
+         if lookup[..|lookup|-1][i].ref == oldchildref && i > 0 && lookup[..|lookup|-1][i-1].ref == parentref && key in movedKeys then newchildref else
+         lookup[..|lookup|-1][i].ref);
+    assert forall i :: 0 <= i < |pref| ==>
+      pref[i].node ==
+        (if lookup[..|lookup|-1][i].ref == parentref then newparent else
+         if lookup[..|lookup|-1][i].ref == oldchildref && i > 0 && lookup[..|lookup|-1][i-1].ref == parentref && key in movedKeys then newchild else
+         lookup[..|lookup|-1][i].node);
+    */
+
+    var accBuf := if |pref| == 0 then [] else pref[|pref| - 1].accumulatedBuffer;
+    var lastLayer := Last(lookup);
+    var ref := 
+      (if lastLayer.ref == parentref then parentref else
+       if lastLayer.ref == oldchildref && |lookup| > 1 && lookup[|lookup|-2].ref == parentref && key in movedKeys then newchildref else
+       lastLayer.ref);
+    var node :=
+      (if lastLayer.ref == parentref then newparent else
+       if lastLayer.ref == oldchildref && |lookup| > 1 && lookup[|lookup|-2].ref == parentref && key in movedKeys then newchild else
+
+       lastLayer.node);
+    pref + [Layer(ref, node, accBuf + (if key in node.buffer then node.buffer[key] else []))]
+  }
+
+  lemma transformLookupParentAndChildLemma<Value>(lookup: Lookup<Value>, lookup': Lookup<Value>, key: Key, parentref: BC.Reference, newparent: Node, movedKeys: iset<Key>, oldchildref: BC.Reference, newchildref: BC.Reference, newchild: Node, i: int)
+  requires 0 <= i < |lookup|
+  requires lookup' == transformLookupParentAndChild(lookup, key, parentref, newparent, movedKeys, oldchildref, newchildref, newchild)
+  ensures
+    lookup'[i].ref ==
+        (if lookup[i].ref == parentref then parentref else
+         if lookup[i].ref == oldchildref && i > 0 && lookup[i-1].ref == parentref && key in movedKeys then newchildref else
+         lookup[i].ref)
+  ensures
+    lookup'[i].node ==
+        (if lookup[i].ref == parentref then newparent else
+         if lookup[i].ref == oldchildref && i > 0 && lookup[i-1].ref == parentref && key in movedKeys then newchild else
+         lookup[i].node)
+  decreases |lookup|
+  {
+    if (i == |lookup| - 1) {
+    } else {
+      transformLookupParentAndChildLemma<Value>(lookup[..|lookup|-1], lookup'[..|lookup|-1],
+          key, parentref, newparent, movedKeys, oldchildref, newchildref, newchild, i);
+    }
+  }
+
+  lemma transformLookupParentAndChildAccumulatesMessages<Value>(lookup: Lookup<Value>, key: Key, parentref: BC.Reference, newparent: Node, movedKeys: iset<Key>, oldchildref: BC.Reference, newchildref: BC.Reference, newchild: Node)
+  requires |lookup| > 0
+  requires LookupVisitsWFNodes(transformLookupParentAndChild(lookup, key, parentref, newparent, movedKeys, oldchildref, newchildref, newchild));
+  ensures LookupAccumulatesMessages(key, transformLookupParentAndChild(lookup, key, parentref, newparent, movedKeys, oldchildref, newchildref, newchild));
+  {
+    var lookup' := transformLookupParentAndChild(lookup, key, parentref, newparent, movedKeys, oldchildref, newchildref, newchild);
+    if (|lookup| == 1) {
+    } else {
+      assert transformLookupParentAndChild(lookup[..|lookup|-1], key, parentref, newparent, movedKeys, oldchildref, newchildref, newchild) ==
+          transformLookupParentAndChild(lookup, key, parentref, newparent, movedKeys, oldchildref, newchildref, newchild)[..|lookup|-1];
+      assert LookupVisitsWFNodes(transformLookupParentAndChild(lookup[..|lookup|-1], key, parentref, newparent, movedKeys, oldchildref, newchildref, newchild));
+
+      transformLookupParentAndChildAccumulatesMessages<Value>(lookup[..|lookup|-1], key, parentref, newparent, movedKeys, oldchildref, newchildref, newchild);
+
+      assert LookupAccumulatesMessages(key, lookup');
+    }
+  }
+
+/*
+  lemma transformLookupParentAndChildLemma<Value>(lookup: Lookup<Value>, key: Key, parentref: BC.Reference, newparent: Node, movedKeys: iset<Key>, oldchildref: BC.Reference, newchildref: BC.Reference, newchild: Node)
+  ensures forall i :: 0 <= i < |lookup| && lookup[i].ref == oldchildref ==>
+      transformLookupParentAndChild(lookup, key, parentref, newparent, movedKeys, oldchildref, newchildref, newchild)[i].ref ==
+        (if lookup[i].ref == parentref then parentref else
+         if lookup[i].ref == oldchildref && i > 0 && lookup[i-1].ref == parentref && key in movedKeys then newchildref else
+         lookup[i].ref)
+  ensures forall i :: 0 <= i < |lookup| ==>
+      transformLookupParentAndChild(lookup, key, parentref, newparent, movedKeys, oldchildref, newchildref, newchild)[i].node ==
+        (if lookup[i].ref == parentref then newparent else
+         if lookup[i].ref == oldchildref && i > 0 && lookup[i-1].ref == parentref && key in movedKeys then newchild else
+         lookup[i].node)
+         *
+  {
+    if (|lookup| == 0) {
+      assume false;
+    } else {
+      var l := lookup[..|lookup|-1];
+      transformLookupParentAndChildLemma<Value>(l, key, parentref, newparent, movedKeys, oldchildref, newchildref, newchild);
+
+          assert forall i :: 0 <= i < |l| ==>
+      transformLookupParentAndChild(l, key, parentref, newparent, movedKeys, oldchildref, newchildref, newchild)[i].ref ==
+        (if l[i].ref == parentref then parentref else
+         if l[i].ref == oldchildref && i > 0 && l[i-1].ref == parentref && key in movedKeys then newchildref else
+         l[i].ref);
+
+      forall i | 0 <= i < |lookup|
+      ensures transformLookupParentAndChild(lookup, key, parentref, newparent, movedKeys, oldchildref, newchildref, newchild)[i].ref ==
+        (if lookup[i].ref == parentref then parentref else
+         if lookup[i].ref == oldchildref && i > 0 && lookup[i-1].ref == parentref && key in movedKeys then newchildref else
+         lookup[i].ref)
+      {
+        if (i < |lookup| - 1) {
+          /*var pref := transformLookupParentAndChild(lookup[.. |lookup| - 1], key, parentref, newparent, movedKeys, oldchildref, newchildref, newchild);
+
+          var accBuf := if |pref| == 0 then [] else pref[|pref| - 1].accumulatedBuffer;
+          var lastLayer := Last(lookup);
+          var ref := 
+            (if lastLayer.ref == parentref then parentref else
+             if lastLayer.ref == oldchildref && |lookup| > 1 && lookup[|lookup|-2].ref == parentref && key in movedKeys then newchildref else
+             lastLayer.ref);
+          var node :=
+            (if lastLayer.ref == parentref then newparent else
+             if lastLayer.ref == oldchildref && |lookup| > 1 && lookup[|lookup|-2].ref == parentref && key in movedKeys then newchild else*/
+
+          assert forall i :: 0 <= i < |lookup[..|lookup|-1]| ==>
+      transformLookupParentAndChild(lookup[..|lookup|-1], key, parentref, newparent, movedKeys, oldchildref, newchildref, newchild)[i].ref ==
+        (if lookup[..|lookup|-1][i].ref == parentref then parentref else
+         if lookup[..|lookup|-1][i].ref == oldchildref && i > 0 && lookup[..|lookup|-1][i-1].ref == parentref && key in movedKeys then newchildref else
+         lookup[..|lookup|-1][i].ref);
+
+
+          assert 0 <= i < |lookup[..|lookup|-1]|;
+
+          var l1 := transformLookupParentAndChild(lookup[..|lookup|-1], key, parentref, newparent, movedKeys, oldchildref, newchildref, newchild);
+          var l2 := transformLookupParentAndChild(lookup, key, parentref, newparent, movedKeys, oldchildref, newchildref, newchild)[..|lookup|-1];
+          assert l1 == l2;
+          assert transformLookupParentAndChild(lookup[..|lookup|-1], key, parentref, newparent, movedKeys, oldchildref, newchildref, newchild)[i].ref
+            ==
+            (if lookup[..|lookup|-1][i].ref == parentref then parentref else
+             if lookup[..|lookup|-1][i].ref == oldchildref && i > 0 && lookup[..|lookup|-1][i-1].ref == parentref && key in movedKeys then newchildref else
+             lookup[..|lookup|-1][i].ref);
+          assert transformLookupParentAndChild(lookup, key, parentref, newparent, movedKeys, oldchildref, newchildref, newchild)[i].ref ==
+            (if lookup[i].ref == parentref then parentref else
+             if lookup[i].ref == oldchildref && i > 0 && lookup[i-1].ref == parentref && key in movedKeys then newchildref else
+             lookup[i].ref);
+        } else {
+          assert transformLookupParentAndChild(lookup, key, parentref, newparent, movedKeys, oldchildref, newchildref, newchild)[i].ref ==
+            (if lookup[i].ref == parentref then parentref else
+             if lookup[i].ref == oldchildref && i > 0 && lookup[i-1].ref == parentref && key in movedKeys then newchildref else
+             lookup[i].ref);
+        }
+      }
+    }
+  }
+  */
+
+  function flushTransformLookup<Value>(lookup: Lookup, key: Key, parentref: BC.Reference, parent: Node, childref: BC.Reference, child: Node, newchildref: BC.Reference) : Lookup
+  requires |lookup| > 0
+  requires WFNode(parent)
+  requires WFNode(child)
+  {
+    var movedKeys := iset k | k in parent.children && parent.children[k] == childref;
+    var newbuffer := imap k :: (if k in movedKeys then parent.buffer[k] + child.buffer[k] else child.buffer[k]);
+    var newchild := Node(child.children, newbuffer);
+    var newparentbuffer := imap k :: (if k in movedKeys then [] else parent.buffer[k]);
+    var newparentchildren := imap k | k in parent.children :: (if k in movedKeys then newchildref else parent.children[k]);
+    var newparent := Node(newparentchildren, newparentbuffer);
+    var lookup1 := if Last(lookup).ref == parentref && key in movedKeys then lookup + [Layer(newchildref, newchild, Last(lookup).accumulatedBuffer + newchild.buffer[key])] else lookup;
+    transformLookupParentAndChild(lookup1, key, parentref, newparent, movedKeys, childref, newchildref, newchild)
+  }
+
+  function flushTransformLookupRev<Value>(lookup': Lookup, key: Key, parentref: BC.Reference, parent: Node, childref: BC.Reference, child: Node, newchildref: BC.Reference) : Lookup
+  {
+    // TODO Use transformLookupParentAndChild instead?
+    // This works fine, but only because newchildref is fresh.
+    // This pattern doesn't work going the other way, so might as well change this one too
+    // for more symmetry.
+    transformLookup(transformLookup(lookup', key, newchildref, childref, child), key, parentref, parentref, parent)
   }
 
   lemma FlushPreservesIsPathFromLookupRev(k: Constants, s: Variables, s': Variables, parentref: BC.Reference, parent: Node, childref: BC.Reference, child: Node, newchildref: BC.Reference, lookup: Lookup, lookup': Lookup, key: Key)
   requires Inv(k, s)
   requires Flush(k, s, s', parentref, parent, childref, child, newchildref)
   requires IsPathFromRootLookup(k, BC.ViewOf(k.bck, s'.bcv), key, lookup')
-  requires lookup == flushTransformLookupRev(lookup', parentref, parent, childref, child, newchildref);
+  requires lookup == flushTransformLookupRev(lookup', key, parentref, parent, childref, child, newchildref);
   ensures IsPathFromRootLookup(k, BC.ViewOf(k.bck, s.bcv), key, lookup);
   // These follow immediately from IsPathFromRootLookup:
   //ensures LookupIsAcyclic(lookup);
@@ -260,7 +480,7 @@ abstract module DiskBetreeInv {
       assert IsPathFromRootLookup(k, BC.ViewOf(k.bck, s.bcv), key, lookup);
     } else {
       FlushPreservesIsPathFromLookupRev(k, s, s', parentref, parent, childref, child, newchildref,
-        flushTransformLookupRev(lookup'[.. |lookup'| - 1], parentref, parent, childref, child, newchildref),
+        flushTransformLookupRev(lookup'[.. |lookup'| - 1], key, parentref, parent, childref, child, newchildref),
         lookup'[.. |lookup'| - 1], key);
 
       assert IsPathFromRootLookup(k, BC.ViewOf(k.bck, s.bcv), key, lookup);
@@ -281,7 +501,7 @@ abstract module DiskBetreeInv {
 
     if (|lookup'| <= 1) {
     } else {
-      var lookup := flushTransformLookupRev(lookup', parentref, parent, childref, child, newchildref);
+      var lookup := flushTransformLookupRev(lookup', key, parentref, parent, childref, child, newchildref);
       FlushPreservesIsPathFromLookupRev(k, s, s', parentref, parent, childref, child, newchildref, lookup, lookup', key);
     }
   }
@@ -330,6 +550,58 @@ abstract module DiskBetreeInv {
     {
       // Remove one for the root
       var lookup := lookup'[1..][0 := Layer(BC.Root(k.bck), lookup'[1].node, lookup'[1].accumulatedBuffer)];
+      assert IsSatisfyingLookup(k, BC.ViewOf(k.bck, s.bcv), key, value, lookup);
+    }
+  }
+
+  lemma FlushEquivalentLookups(k: Constants, s: Variables, s': Variables, parentref: BC.Reference, parent: Node, childref: BC.Reference, child: Node, newchildref: BC.Reference)
+  requires Inv(k, s)
+  requires Flush(k, s, s', parentref, parent, childref, child, newchildref)
+  ensures EquivalentLookups(k, s, s')
+  {
+    forall lookup:Lookup, key, value | IsSatisfyingLookup(k, BC.ViewOf(k.bck, s.bcv), key, value, lookup)
+    ensures exists lookup' :: IsSatisfyingLookup(k, BC.ViewOf(k.bck, s'.bcv), key, value, lookup')
+    {
+      var movedKeys := iset k | k in parent.children && parent.children[k] == childref;
+      var newbuffer := imap k :: (if k in movedKeys then parent.buffer[k] + child.buffer[k] else child.buffer[k]);
+      var newchild := Node(child.children, newbuffer);
+      var newparentbuffer := imap k :: (if k in movedKeys then [] else parent.buffer[k]);
+      var newparentchildren := imap k | k in parent.children :: (if k in movedKeys then newchildref else parent.children[k]);
+      var newparent := Node(newparentchildren, newparentbuffer);
+      var lookup1 := if Last(lookup).ref == parentref && key in movedKeys then lookup + [Layer(newchildref, newchild, Last(lookup).accumulatedBuffer + newchild.buffer[key])] else lookup;
+
+      var lookup' := flushTransformLookup(lookup, key, parentref, parent, childref, child, newchildref);
+
+      transformLookupParentAndChildLemma(lookup1, lookup', key, parentref, newparent, movedKeys, childref, newchildref, newchild, 0);
+
+      assert lookup'[0].ref == BC.Root(k.bck);
+
+      forall i | 0 <= i < |lookup'|
+      ensures IMapsTo(BC.ViewOf(k.bck, s'.bcv), lookup'[i].ref, lookup'[i].node)
+      ensures WFNode(lookup'[i].node)
+      {
+        transformLookupParentAndChildLemma(lookup1, lookup', key, parentref, newparent, movedKeys, childref, newchildref, newchild, i);
+      }
+
+      forall i | 0 <= i < |lookup'| - 1
+      ensures key in lookup'[i].node.children
+      ensures lookup'[i].node.children[key] == lookup'[i+1].ref
+      {
+        transformLookupParentAndChildLemma(lookup1, lookup', key, parentref, newparent, movedKeys, childref, newchildref, newchild, i);
+        transformLookupParentAndChildLemma(lookup1, lookup', key, parentref, newparent, movedKeys, childref, newchildref, newchild, i+1);
+      }
+
+      transformLookupParentAndChildAccumulatesMessages(lookup1, key, parentref, newparent, movedKeys, childref, newchildref, newchild);
+
+      assert IsSatisfyingLookup(k, BC.ViewOf(k.bck, s'.bcv), key, value, lookup');
+    }
+
+    forall lookup': Lookup, key, value | IsSatisfyingLookup(k, BC.ViewOf(k.bck, s'.bcv), key, value, lookup')
+    ensures exists lookup :: IsSatisfyingLookup(k, BC.ViewOf(k.bck, s.bcv), key, value, lookup)
+    {
+      var lookup := flushTransformLookupRev(lookup', key, parentref, parent, childref, child, newchildref);
+      FlushPreservesIsPathFromLookupRev(k, s, s', parentref, parent, childref, child, newchildref, lookup, lookup', key);
+      transformLookupAccumulatesMessages(transformLookup(lookup', key, newchildref, childref, child), key, parentref, parentref, parent);
       assert IsSatisfyingLookup(k, BC.ViewOf(k.bck, s.bcv), key, value, lookup);
     }
   }
